\documentclass[a4paper, 20pt]{article}
\usepackage[utf8]{inputenc}
\usepackage{paralist}
\usepackage{jeffe,handout}
\usepackage{eqarrays}
\usepackage{tikz}
\usetikzlibrary{matrix}
\usetikzlibrary{arrows,shapes.gates.logic.US,shapes.gates.logic.IEC,calc}
\usepackage{hyperref}
\usepackage{aurical}
\usepackage[T1]{fontenc}

\def\lnot{\mathop{\sim}}
\def\implies{\mathop{\rightarrow}}
\def\xor{\mathop{\oplus}}
\def\iff{\mathop{\leftrightarrow}}

\begin{document}
\headers{CPSC 121}{ }{2019S}

\begin{center}
    \LARGE
    \textbf{HW 1}
    \\[1ex]
    \Large Due: Wednesday, May 15, 2019 at 23:00 \\
\end{center}
    \LARGE
\begin{tabular}{rl}
 & \\
CSID 1: & d6a2b\\
 & \\
CSID 2: & b9i2b\\
 & \\
\end{tabular}
\large

\textbf{Instructions:}
\begin{enumerate}
\item Do not change the problem statements we are giving you. Simply add your solutions by editing this latex document. 
\item If you need more space, add a page between the existing pages using the \texttt{\textbackslash newpage} command.
\item Where possible, include formatting to clearly distinguish your solutions from the given problem text (e.g. use a different font colour for your solutions).
\item Export the completed assignment as a PDF file for upload to gradescope.
\item On Gradescope, upload only \textbf{one} copy per partnership. (Instructions for uploading to Gradescope are posted on the assignments page of the course website.)
\item Late submissions will be accepted up to 24 hours past the deadline with a penalty of 20\% of the assignment's maximum value.
\end{enumerate}

\textbf{Academic Conduct:} 
I certify that my assignment follows the academic conduct rules for of CPSC 121 as outlined on the course website. As part of those rules, when collaborating with anyone outside my group, (1) I and my collaborators took no record but names away, and (2) after a suitable break, my group created the assignment I am submitting without help from anyone other than the course staff. \\

\textbf{Version history:}
\begin{itemize}
    \item 2019-05-08 16:15 -- parenthesis added in Q1a; Q3 gate limit relaxed slightly
    \item 2019-05-05 20:31 -- Initial version for release
\end{itemize}

\newpage
\begin{question}{1.}
\input{prob1.tex}
\newpage
\\1(a).
\\ Proof:
\\ $\equiv \lnot p \land q \land (\lnot s \lor (\lnot r \land s)) \lor (q \land(p \lor (\lnot p \land r \land s)))$ [Start]
\\ $\equiv \lnot p \land q \land (\lnot s \lor (\lnot r \land s)) \lor (q \land((p \lor \lnot p) \land(p \lor r) \land(p \lor s)))$ [DIST]
\\ $\equiv (\lnot p \land q \land ((\lnot s \lor \lnot r) \land (\lnot s \lor s))) \lor (q \land((p \lor \lnot p) \land(p \lor r) \land(p \lor s)))$ [DIST]
\\ $\equiv (\lnot p \land q \land ((\lnot s \lor \lnot r) \land T)) \lor (q \land((p \lor \lnot p) \land(p \lor r) \land(p \lor s)))$ [NEG]
\\ $\equiv (\lnot p \land q \land ((\lnot s \lor \lnot r) \land T)) \lor (q \land(T \land(p \lor r) \land(p \lor s)))$ [NEG]
\\ $\equiv (\lnot p \land q \land (\lnot s \lor \lnot r)) \lor (q \land(T \land(p \lor r) \land(p \lor s)))$ [I]
\\ $\equiv (\lnot p \land q \land (\lnot s \lor \lnot r)) \lor (q \land(p \lor r) \land(p \lor s))$ [I]
\\ $\equiv (q \land \lnot p \land (\lnot s \lor \lnot r)) \lor (q \land(p \lor r) \land(p \lor s))$ [COM]
\\ $\equiv q \land ((\lnot p \land (\lnot s \lor \lnot r)) \lor ((p \lor r) \land(p \lor s)))$ [DIST]
\\ $\equiv q \land ((\lnot p \land (\lnot s \lor \lnot r)) \lor (p \lor (r \land s)))$ [DIST]
\\ $\equiv q \land ((\lnot p \land \lnot (s \land r)) \lor (p \lor (r \land s)))$ [DM]
\\ $\equiv q \land (\lnot (p \lor (s \land r)) \lor (p \lor (r \land s)))$ [DM]
\\ $\equiv q \land (\lnot (p \lor (r \land s)) \lor (p \lor (r \land s)))$ [COM]
\\ $\equiv q \land T$ [NEG]
\\ $\equiv q$ [I]
\\ \boxed{}
\\
\\
\\1(b).
\\ Proof:
\\ $\equiv ((w \land x)\lor(\lnot w \land \lnot x))\land((\lnot y \land \lnot z)\lor(y \land z))\lor \lnot(w \land y)$ [Start]
\\ $\equiv (((w \land x)\lor(\lnot w \land \lnot x))\land((\lnot y \land \lnot z)\lor(y \land z)))\lor \lnot w \lor \lnot y$ [DM]
\\ $\equiv (((w \land x)\lor(\lnot w \land \lnot x))\lor \lnot w \land((\lnot y \land \lnot z)\lor(y \land z))\lor \lnot w ) \lor \lnot y$ [DIST]
\\ $\equiv (((w \land x)\lor(\lnot w \land \lnot x)\lor \lnot w) \land((\lnot y \land \lnot z)\lor(y \land z))\lor \lnot w ) \lor \lnot y$ [ASS]
\\ $\equiv (((w \land x)\lor \lnot w \lor (\lnot w \land \lnot x)) \land((\lnot y \land \lnot z)\lor(y \land z))\lor \lnot w ) \lor \lnot y$ [COM]
\\ $\equiv ((((w \lor \lnot w) \land (x \lor \lnot w)) \lor (\lnot w \land \lnot x)) \land((\lnot y \land \lnot z)\lor(y \land z))\lor \lnot w ) \lor \lnot y$ [DIST]
\\ $\equiv (((T \land (x \lor \lnot w)) \lor (\lnot w \land \lnot x)) \land((\lnot y \land \lnot z)\lor(y \land z))\lor \lnot w ) \lor \lnot y$ [NEG]
\\ $\equiv ((((x \lor \lnot w)) \lor (\lnot w \land \lnot x)) \land((\lnot y \land \lnot z)\lor(y \land z))\lor \lnot w ) \lor \lnot y$ [I]
\\ $\equiv ((((\lnot w \lor x)) \lor (\lnot w \land \lnot x)) \land((\lnot y \land \lnot z)\lor(y \land z))\lor \lnot w ) \lor \lnot y$ [COM]
\\ $\equiv ((\lnot w \lor x \lor (\lnot w \land \lnot x)) \land((\lnot y \land \lnot z)\lor(y \land z))\lor \lnot w ) \lor \lnot y$ [ASS]
\\ $\equiv ((\lnot w \lor (x \lor \lnot w \land x \lor \lnot x)) \land((\lnot y \land \lnot z)\lor(y \land z))\lor \lnot w ) \lor \lnot y$ [DIST]
\\ $\equiv ((\lnot w \lor (x \lor \lnot w \land T)) \land((\lnot y \land \lnot z)\lor(y \land z))\lor \lnot w ) \lor \lnot y$ [NEG]
\\ $\equiv ((\lnot w \lor (x \lor \lnot w)) \land((\lnot y \land \lnot z)\lor(y \land z))\lor \lnot w ) \lor \lnot y$ [I]
\\ $\equiv ((\lnot w \lor x \lor \lnot w) \land((\lnot y \land \lnot z)\lor(y \land z))\lor \lnot w ) \lor \lnot y$ [ASS]
\\ $\equiv ((\lnot w \lor \lnot w \lor x ) \land((\lnot y \land \lnot z)\lor(y \land z))\lor \lnot w ) \lor \lnot y$ [COM]
\\ $\equiv ((\lnot w \lor x ) \land((\lnot y \land \lnot z)\lor(y \land z))\lor \lnot w ) \lor \lnot y$ [ID]
\\ $\equiv ((\lnot w \lor x ) \land \lnot w \lor((\lnot y \land \lnot z)\lor(y \land z)) ) \lor \lnot y$ [COM]
\\ $\equiv \lnot w \lor( x \land((\lnot y \land \lnot z)\lor(y \land z)) ) \lor \lnot y$ [DIST]
\\ $\equiv \lnot w \lor(x \lor \lnot y \land((\lnot y \land \lnot z)\lor(y \land z)) \lor \lnot y ) $ [DIST]
\\ $\equiv \lnot w \lor((x \lor \lnot y) \land((\lnot y \land \lnot z)\lor(y \land z)) \lor \lnot y ) $ [ASS]
\\ $\equiv \lnot w \lor((x \lor \lnot y) \land((\lnot y \land \lnot z)\lor(y \land z) \lor \lnot y )) $ [ASS]
\\ $\equiv \lnot w \lor((x \lor \lnot y) \land((\lnot y \land \lnot z)\lor((y \lor \lnot y) \land (z \lor \lnot y )))) $ [DIST]
\\ $\equiv \lnot w \lor((x \lor \lnot y) \land((\lnot y \land \lnot z)\lor(T \land (z \lor \lnot y )))) $ [NEG]
\\ $\equiv \lnot w \lor((x \lor \lnot y) \land((\lnot y \land \lnot z)\lor((z \lor \lnot y )))) $ [I]
\\ $\equiv \lnot w \lor((x \lor \lnot y) \land((\lnot y \land \lnot z)\lor z \lor \lnot y )) $ [ASS]
\\ $\equiv \lnot w \lor((x \lor \lnot y) \land((\lnot y \lor z) \land (\lnot z \lor z) \lor \lnot y )) $ [ASS]
\\ $\equiv \lnot w \lor((x \lor \lnot y) \land((\lnot y \lor z) \land (\lnot z \lor z) \lor \lnot y )) $ [DIST]
\\ $\equiv \lnot w \lor((x \lor \lnot y) \land((\lnot y \lor z) \land T \lor \lnot y )) $ [NEG]
\\ $\equiv \lnot w \lor((x \lor \lnot y) \land((\lnot y \lor z)  \lor \lnot y )) $ [I]
\\ $\equiv \lnot w \lor((x \lor \lnot y) \land(\lnot y \lor z  \lor \lnot y )) $ [ASS]
\\ $\equiv \lnot w \lor((x \lor \lnot y) \land( z \lor \lnot y \lor \lnot y )) $ [COM]
\\ $\equiv \lnot w \lor((x \lor \lnot y) \land( z \lor \lnot y )) $ [COM]
\\ $\equiv \lnot w \lor(x  \land z)\lor \lnot y $ [DIST]
\\ \boxed{}
\newpage
\input{prob2.tex}
\\2(a). B \equiv D
\\ expression 1, expression 2, reason
\\$(\lnot a \lor b)\land(\lnot a \lor c)\land(\lnot a \lor \lnot d) \equiv a \implies (b \land c \land \lnot d)$ [Start]
\\$(\lnot a \lor b)\land(\lnot a \lor c)\land(\lnot a \lor \lnot d) \equiv \lnot a \lor (b \land c \land \lnot d)$ [IMP]
\\$\lnot a \lor (b \land c \land \lnot d) \equiv \lnot a \lor (b \land c \land \lnot d)$ [DIST]
\\
\\2(b). A \equiv E
\\ expression 1, expression 2, reason
\\$ (\lnot a \land b) \iff \lnot(c \lor d) \equiv \lnot ((a \lor \lnot b \lor c \lor d) \land ((\lnot a \land b) \lor \lnot (c \lor d)))$ [Start]
\\$ \lnot ((\lnot a \land b) (+) \lnot(c \lor d)) \equiv \lnot ((a \lor \lnot b \lor c \lor d) \land ((\lnot a \land b) \lor \lnot (c \lor d)))$ [Equivalence definition]
\\$  \lnot (\lnot ((\lnot a \land b) \land \lnot (c \lor d)) \land ((\lnot a \land b) \lor \lnot (c \lor d))) \equiv \lnot ((a \lor \lnot b \lor c \lor d) \land ((\lnot a \land b) \lor \lnot (c \lor d)))$ [Xor definition]
\\$  \lnot (\lnot ((\lnot a \land b) \land \lnot (c \lor d)) \land ((\lnot a \land b) \lor \lnot (c \lor d))) \equiv \lnot ((\lnot( \lnot a \land b) \lor c \lor d) \land ((\lnot a \land b) \lor \lnot (c \lor d)))$ [DM]
\\$  \lnot (\lnot ((\lnot a \land b) \land \lnot (c \lor d)) \land ((\lnot a \land b) \lor \lnot (c \lor d))) \equiv \lnot ((\lnot( \lnot a \land b) \lor (c \lor d)) \land ((\lnot a \land b) \lor \lnot (c \lor d)))$ [ASS]
\\$  \lnot (\lnot ((\lnot a \land b) \land \lnot (c \lor d)) \land ((\lnot a \land b) \lor \lnot (c \lor d))) \equiv \lnot (\lnot(( \lnot a \land b) \land \lnot (c \lor d)) \land ((\lnot a \land b) \lor \lnot (c \lor d)))$ [DM]
\\
\\3(c). C $\equiv$ F
\\ Truth table of C:
\\
\begin{displaymath}
\begin{array}{|c c c c|c|c|c|}
a & b & c & d & (a \land b \land c)&\lnot(b \land c \land d)&f \equiv (a \land b \land c)\lor \lnot(b \land c \land d)\\
\hline 
1&1&1&X&1&X&1\\
X&0&X&X&X&1&1\\
X&X&0&X&X&1&1\\
X&X&X&0&X&1&1\\
\end{array}
\end{displaymath}
\\ Since the statement is separated by an Or gate, we can find what makes either terms true and ignore the other term. That lets us deduce the truth table quickly. Unmentioned input combination(s) is false.
\\
\\ Truth table of F:
\\
\begin{displaymath}
\begin{array}{|c c c c|c|c|c|c|c|}
a & b & c & d & w \equiv (c (+) d) & x \equiv \lnot (a (+) b) & y \equiv \lnot (c \lor d) & z \equiv (a \land \lnot b) & f = w \lor x \lor y \lor z\\
\hline 
0 & 0 & 0 & 0 &0&1&1&0&1\\
0 & 0 & 0 & 1 &1&1&0&0&1\\
0 & 0 & 1 & 0 &1&1&0&0&1\\
0 & 0 & 1 & 1 &0&1&0&0&1\\
0 & 1 & 0 & 0 &0&0&1&0&1\\
0 & 1 & 0 & 1 &1&0&0&0&1\\
0 & 1 & 1 & 0 &1&0&0&0&1\\
0 & 1 & 1 & 1 &0&0&0&0&0\\
1 & 0 & 0 & 0 &0&0&1&1&1\\
1 & 0 & 0 & 1 &1&0&0&1&1\\
1 & 0 & 1 & 0 &1&0&0&1&1\\
1 & 0 & 1 & 1 &0&0&0&1&1\\
1 & 1 & 0 & 0 &0&1&1&0&1\\
1 & 1 & 0 & 1 &1&1&0&0&1\\
1 & 1 & 1 & 0 &1&1&0&0&1\\
1 & 1 & 1 & 1 &0&1&0&0&1\\
\end{array}
\end{displaymath}
\\
\\ These two truth tables' output values are the same for given input value (ie only 0111 input makes output 0), therefore the two logical statements are equivalent.
\newpage
\input{prob3.tex}
\newpage
\\3(a).
\\
\leavevmode\lower45pt\hbox{\includegraphics[scale=0.75]{3a.jpg}}
\\Proof:
\\ $ \equiv \lnot (a \lor a)$ [Start]
\\ $ \equiv \lnot (a)$ [ID]
\\ $ \equiv \lnot a$ [ASS]
\\ \boxed{}
\\
\\3(b).
\\
\leavevmode\lower45pt\hbox{\includegraphics[scale=0.75]{3b.jpg}}
\\ Proof:
\\ $ \equiv \lnot (\lnot (a \lor b) \lor \lnot (a \lor b))$ [Start]
\\ $ \equiv \lnot (\lnot (a \lor b))$ [ID]
\\ $ \equiv (a \lor b)$ [DNEG]
\\ \boxed{}
\\
\\3(c).
\\
\leavevmode\lower45pt\hbox{\includegraphics[scale=0.75]{3c.jpg}}
\begin{displaymath}
\begin{array}{|c c|c|c|c|c|}
a & b & \lnot (a \lor a) \equiv \lnot a & \lnot (b \lor b) \equiv \lnot b & \lnot (\lnot (a \lor a) \lor \lnot (b \lor b)) \equiv \lnot (\lnot a \lor \lnot b) & a \land b\\
\hline 
0 & 0 & 1 & 1 & 0 & 0\\
0 & 1 & 1 & 0 & 0 & 0\\
1 & 0 & 0 & 1 & 0 & 0\\
1 & 1 & 0 & 0 & 1 & 1\\
\end{array}
\end{displaymath}
\\3(d).
\\ Since the question didn't specify how we should simplify the truth table, I will use K-map for simplicity:
\begin{displaymath}
\begin{array}{|c|c|c|c|c|}
- & x1 \land x0 & \lnot x1 \land x0 & \lnot x1 \land \lnot x0 & x1 \land \lnot x0 \\
\hline 
x3 \land x2 & 0&1&1&0\\
\lnot x3 \land x2 & 0&0&1&0\\
\lnot x3 \land \lnot x2 & 0&0&0&1\\
x3 \land \lnot x2 & 0&0&0&1\\
\end{array}
\end{displaymath}
\\ Finding sum of minterms, I can get:
\\ $f \equiv (x2 \land \lnot x1 \land \lnot x0) \lor (x3 \land x2 \land \lnot x1) \lor (\lnot x2 \land x1 \land \lnot x0)$
\\
\\ I can use logical properties to change the logical statement into one that's made up of only Nor gates:
\\
\\ Proof:
\\ $\equiv (x2 \land \lnot x1 \land \lnot x0) \lor (x3 \land x2 \land \lnot x1) \lor (\lnot x2 \land x1 \land \lnot x0)$ [Start]
\\ $\equiv \lnot (\lnot x2 \lor x1 \lor x0) \lor \lnot (\lnot x3 \lor \lnot x2 \lor x1) \lor \lnot (x2 \lor \lnot x1 \lor x0)$ [DM to all And terms]
\\ $\equiv \lnot (\lnot (x2 \lor x2) \lor x1 \lor x0) \lor \lnot (\lnot (x3 \lor x3) \lor \lnot (x2 \lor x2) \lor x1) \lor \lnot (x2 \lor \lnot (x1 \lor x1) \lor x0)$ [ID to all Not terms]
\\ $\equiv \lnot (\lnot (\lnot (\lnot (x2 \lor x2) \lor x1 \lor x0) \lor \lnot (\lnot (x3 \lor x3) \lor \lnot (x2 \lor x2) \lor x1) \lor \lnot (x2 \lor \lnot (x1 \lor x1) \lor x0)))$ [DNEG]
\\ \boxed{}
\\
\\ This logical statement can be simplified further, but it already uses under 16 gates, as shown here:
\\ 
\leavevmode\lower45pt\hbox{\includegraphics[scale=0.75]{3d.jpg}}
\newpage
\input{prob4.tex}
\newpage
\\ 4.
\\ I know that in the range of [0, 31] the prime numbers are:  2, 3, 5, 7, 11, 13, 17, 19, 23, 29, 31. I can write a truth table from these outputs. 
\begin{displaymath}
\begin{array}{|c c c c c|c|c|}
x4&x3&x2&x1&x0&Decimal&z\\
\hline 
0 & 0 & 0 & 0 & 0 & 0&0\\
0 & 0 & 0 & 0 & 1 & 1&0\\
0 & 0 & 0 & 1 & 0 & 2&1\\
0 & 0 & 0 & 1 & 1 &3&1\\
0 & 0 & 1 & 0 & 0 &4&0\\
0 & 0 & 1 & 0 & 1 &5&1\\
0 & 0 & 1 & 1 & 0 &6&0\\
0 & 0 & 1 & 1 & 1 &7&1\\
0 & 1 & 0 & 0 & 0 &8&0\\
0 & 1 & 0 & 0 & 1 &9&0\\
0 & 1 & 0 & 1 & 0 &10&0\\
0 & 1 & 0 & 1 & 1 &11&1\\
0 & 1 & 1 & 0 & 0 &12&0\\
0 & 1 & 1 & 0 & 1 &13&1\\
0 & 1 & 1 & 1 & 0 &14&0\\
0 & 1 & 1 & 1 & 1 &15&0\\
1 & 0 & 0 & 0 & 0 &16&0\\
1 & 0 & 0 & 0 & 1 &17&1\\
1 & 0 & 0 & 1 & 0 &18&0\\
1 & 0 & 0 & 1 & 1 &19&1\\
1 & 0 & 1 & 0 & 0 &20&0\\
1 & 0 & 1 & 0 & 1 &21&0\\
1 & 0 & 1 & 1 & 0 &22&0\\
1 & 0 & 1 & 1 & 1 &23&1\\
1 & 1 & 0 & 0 & 0 &24&0\\
1 & 1 & 0 & 0 & 1 &25&0\\
1 & 1 & 0 & 1 & 0 &26&0\\
1 & 1 & 0 & 1 & 1 &27&0\\
1 & 1 & 1 & 0 & 0 &28&0\\
1 & 1 & 1 & 0 & 1 &29&1\\
1 & 1 & 1 & 1 & 0 &30&0\\
1 & 1 & 1 & 1 & 1 &31&1\\
\end{array}
\end{displaymath}
\\ Since the question did not specify the method, I can use K-map made from this truth table to get logical statement of $z$:
\\
\begin{displaymath}
\begin{array}{|c|c|c|c|c|}
- & x1 \land x0 & \lnot x1 \land x0 & \lnot x1 \land \lnot x0 & x1 \land \lnot x0 \\
\hline 
x4 \land x3 \land x2 & 1&1&0&0\\
x4 \land \lnot x3 \land x2 & 1&0&0&0\\
x4 \land \lnot x3 \land \lnot x2 & 1&1&0&0\\
x4 \land x3 \land \lnot x2 & 0&0&0&0\\
\lnot x4 \land x3 \land \lnot x2 & 1&0&0&0\\
\lnot x4 \land \lnot x3 \land \lnot x2 & 1&0&0&1\\
\lnot x4 \land \lnot x3 \land x2 & 1&1&0&0\\
\lnot x4 \land x3 \land x2 & 0&1&0&0\\
\end{array}
\end{displaymath}
\\
\\ We can rewrite these two K-maps into logical statements as follow:
\\ $ z = (x3 \land x2 \land \lnot x1 \land x0) \lor (\lnot x4 \land \lnot x3 \land x2 \land x0) \lor (\lnot x4 \land \lnot x3 \land \lnot x2 \land x1) \lor (\lnot x4 \land \lnot x2 \land x1 \land x0) \lor (x4 \land \lnot x3 \land \lnot x2 \land x0) \lor (x4 \land x2 \land x1 \land x0) $
\\
\\ Using K-map, we can be sure that this is the most simplified form of the logical statement. While there are one Xor and one Xnor simplifications we can make with $(4(+)2)$ and $\lnot (4(+)2)$, it doesn't decrease the number of logic gates since we still need to wrap the Xor and Xnor with an And gate (respectively) to pair it with other terms ($(\lnot x3 \land x0)$ and $(x1 \land x0)$, respectively). We can make this into a logic circuit:
\\
\leavevmode\lower45pt\hbox{\includegraphics[scale=0.75]{4.PNG}}
\\
\\ Note that I have to use two separate Or gates at the output since Logisim has 5 input maximum for their Or gate.
\\
\\ 
\end{question}
\end{document}