\item[8] Apply the rules of logical equivalence to reduce the following expressions to the indicated number of literals. Recall that a literal is one Boolean variable or its negation. Show your intermediate steps.

\begin{enumerate}
    \item $\lnot p \land q \land (\lnot s \lor (\lnot r \land s)) \lor (q \land(p \lor (\lnot p \land r \land s)))$, to 1 literal
    \vspace{3.0in}
    \item $((w \land x)\lor(\lnot w \land \lnot x))\land((\lnot y \land \lnot z)\lor(y \land z))\lor \lnot(w \land y)$, to 4 literals
    \vspace{3.0in}
\end{enumerate}

\newpage